src/3d/GeneralizeProbes.fsti
@@ -16,7 +16,6 @@
 module GeneralizeProbes
 open FStar.All
 open Ast
-val simple_probe_function_for_type (t:ident) : ML ident 
-val ungeneralize_name (t:ident) : ML ident
+val simple_probe_function_for_type (t:ident) : ident 
 val generalize_probe_decls (e:GlobalEnv.global_env) (ds:list decl)
 : ML (list decl)
